\documentclass[12pt, a4paper]{article}
\usepackage{enumitem}
\setlist[enumerate]{label = (\roman*)}
\usepackage{amsmath}
\usepackage{mathtools}
\usepackage{amssymb}
\usepackage{amsthm}
\theoremstyle{definition}
\newtheorem{example}{Example}

\usepackage{tikz}
\usepackage{hyperref}

\newcommand{\summation}[2]{\sum\limits_{#1}^{#2}}
\newcommand{\limit}[2]{\lim\limits_{#1\to #2}}
\newcommand{\vep}{\varepsilon}

\begin{document}
\begin{example}[$\frac{\partial \tilde{\beta}'A\tilde{\beta}}{\partial \tilde{\beta}}=2A\tilde{\beta}$]
Consider $\tilde{\beta}$ and matrix $A$ as following,
\[
 \tilde{\beta}=[\tilde{\beta_1},\tilde{\beta_2},\dots,\tilde{\beta_k}]^{'},
 A=\begin{bmatrix}
 a_{11} & a_{12} & \dots & a_{1k} \\
 a_{21} & a_{22} & \dots & a_{2k} \\
 \vdots & \dots & \ddots & \vdots \\
 a_{k1} & a_{k2} & \dots & a_{kk}
 \end{bmatrix} \forall{i,j}, a_{ij}=a_{ji}
\]
Then, $\frac{\partial \tilde{\beta}'A\tilde{\beta}}{\partial \tilde{\beta}}=2A\tilde{\beta}$.

 
\begin{proof} 
Notice that
\[
 \tilde{\beta}^{'}A = [\tilde{\beta_1},\tilde{\beta_2},\dots,\tilde{\beta_k}] \times \begin{bmatrix}
 a_{11} & a_{12} & \dots & a_{1k} \\
 a_{21} & a_{22} & \dots & a_{2k} \\
 \vdots & \dots & \ddots & \vdots \\
 a_{k1} & a_{k2} & \dots & a_{kk}
 \end{bmatrix} = \begin{bmatrix}
 \sum\limits_{i=1}^k \tilde{\beta_i}a_{i1}, \sum\limits_{i=1}^k \tilde{\beta_i}a_{i2},\dots, \sum\limits_{i=1}^k \tilde{\beta_i}a_{ik}
 \end{bmatrix} 
 \]
Hence,
\begin{align*}
 \tilde{\beta}^{'}A\tilde{\beta} &= \begin{bmatrix}
 \sum\limits_{i=1}^k \tilde{\beta_i}a_{i1}, \sum\limits_{i=1}^k \tilde{\beta_i}a_{i2},\dots, \sum\limits_{i=1}^k \tilde{\beta_i}a_{ik}
 \end{bmatrix} \begin{bmatrix}
 \tilde{\beta_1}\\
 \tilde{\beta_2}\\
 \vdots\\
 \tilde{\beta_k}
 \end{bmatrix} \\
 &= (\tilde{\beta_1}^2a_{11}+\tilde{\beta_2}^2a_{22}+\dots+\tilde{\beta_k}^2a_{kk})+(\sum\limits_{i\neq1}^k \tilde{\beta_i}a_{i1})\tilde{\beta_1}+
 (\sum\limits_{i\neq2}^k \tilde{\beta_i}a_{i2})\tilde{\beta_2}+
 \dots+(\sum\limits_{i\neq k}^k \tilde{\beta_i}a_{ik})\tilde{\beta_k}
 \end{align*}
 Therefore, 
 \begin{align*}
 \frac{\partial{\tilde{\beta}^{'}A\tilde{\beta}}}{\partial{\tilde{\beta_j}}} &=
 2\tilde{\beta_j}a_{jj}+\tilde{\beta_1}a_{j1}+\tilde{\beta_2}a_{j2}+\dots+\tilde{\beta}_{j-1}a_{j,j-1}+
 \sum\limits_{i\neq j}^k \tilde{\beta_i}a_{ij}+\dots+\tilde{\beta_k}a_{jk} \\
  &= 2\tilde{\beta_j}a_{jj}+\tilde{\beta_1}a_{j1}+\tilde{\beta_2}a_{j2}+\dots+\tilde{\beta}_{j-1}a_{j,j-1}+
 \sum\limits_{i\neq j}^k \tilde{\beta_i}a_{ji}+\dots+\tilde{\beta_k}a_{jk} \\
 &= 2(\tilde{\beta_1}a_{j1}+\tilde{\beta_2}a_{j2}+\dots+\tilde{\beta_k}a_{jk})=2[a_{j1},a_{j2},\dots,a_{jk}]
 \begin{bmatrix}
 \tilde{\beta_1}\\
 \tilde{\beta_2}\\
 \vdots\\
 \tilde{\beta_k}
 \end{bmatrix}
 \end{align*}
\end{proof}
\end{example}

\begin{example}[$\sigma^{-2}(n-K)s_{UB}^2\sim\chi^2(n-K)$]
To prove: 
\[
\sigma^{-2}(n-K)s_{UB}^2\sim \chi^2(n-K)
\]
we need to following two facts:
\begin{enumerate}
\item If random vector \textbf{x} $\sim N(\textbf{0},\textbf{I}_n)$ and $\bold{A}$ is idempotent matrix, then $\bold{x'Ax}\sim \chi^2$(rank($\bold{A}$)), where rank($\bold{A}$) is the degree of freedom of this chi-square distribution.
\item For an idempotent matrix $M$, we have: rank($M$) = trace($M$).
\end{enumerate}
\begin{proof}
Assume we have known these two facts, let's begin to prove it:
\begin{align*}
\sigma^{-2}(n-K)s_{UB}^2 &= \frac{\sum\limits_{i=1}^n (\hat{\vep_i}^2)}{\sigma^2}\\
& = \frac{\hat{\vep}'\cdot \hat{\vep}}{\sigma^2} \\
& = \frac{(Y-\hat{Y})'(Y-\hat{Y})}{\sigma^2} \\
&= \frac{(Y-X\hat{\beta})'(Y-X\hat{\beta})}{\sigma^2}\\
&= \frac{(Y-X(X'X)^{-1}X'Y)'(Y-X(X'X)^{-1}X'Y)}{\sigma^2} \\
&= \frac{[(I_n-X(X'X)^{-1}X')Y]'[(I_n-X(X'X)^{-1}X')Y]}{\sigma^2} 
\end{align*}
Recall that
\[
M = I_n-X(X'X)^{-1}X' = I_n - P. 
\]
Hence, 
\begin{align*}
\sigma^{-2}(n-K)s_{UB}^2 &=\frac{(MY)'(MY)}{\sigma^2}\\
&= \frac{[M(X\beta +\vep)]'[M(X\beta +\vep)]}{\sigma^2}\\
&=\frac{[(I_n-P)X\beta + M\vep]'[(I_n-P)X\beta + M\vep]}{\sigma^2}
\end{align*}
Notice that: 
\[
(I_n-P)X\beta + M\vep = (I_n - X(X'X)^{-1}X')X\beta + M\vep=M\vep
\]
Hence, 
\[
\sigma^{-2}(n-K)s_{UB}^2 =\frac{(M\vep)'(M\vep)}{\sigma^2}
\]
$M$ is idempotent implies 
\[
\sigma^{-2}(n-K)s_{UB}^2 = \frac{\vep'M\vep}{\sigma^2} = \frac{\vep'}{\sigma}M\frac{\vep}{\sigma}
\]
By fact (i), we can assert that: $\sigma^{-2}(n-K)s_{UB}^2 \sim \chi^2$(rank($M$)), now we need to show: rank($M$) = $n-K$. By fact (ii), we need to show: trace($M$) = $n-K$.
\begin{align*}
trace(M) &= trace(I_n - X(X'X)^{-1}X')\\
&= trace(I_n) - trace(X(X'X)^{-1}X')
\end{align*}
As $trace(AB) = trace(BA)$, hence
\begin{align*}
trace(M)&= n-trace((X'X)^{-1}X'X)\\
&=n-K
\end{align*}
\end{proof}

\end{example}


























\end{document}